Insert error

SQL1.thy
@@ -1,16 +1,16 @@
 theory SQL1
-  imports Main
+  imports Main "~~/src/HOL/Library/Finite_Map"
 begin
 
 
 
 datatype s_type = ST_String | ST_Int | ST_Date
 
-datatype s_rowname = SRN_String string
+type_synonym s_rowname = string
 
 datatype s_value = SV_String string | SV_Int int | SV_Null
 
-datatype s_schema = SS_Schema "(s_rowname * s_type) list"
+datatype s_schema = SS_Schema "(s_rowname, s_type) fmap"
 
 datatype s_select_argument = SSA_Rowname s_rowname | SSA_Star
 
@@ -22,66 +22,97 @@ datatype s_where_argument = SWA_AND s_where_argument s_where_argument | SWA_ISNU
 
 datatype s_group_by = SGB_Empty
 
-datatype s_row = SS_Row "(s_select_argument * s_value) list"
+datatype s_row = SS_Row "(s_select_argument, s_value) fmap"
 
-datatype s_query_result = SQR "s_row list"
+datatype s_query_result = SQR_Success "s_row list" | SQR_Error string
 
-datatype s_query = SQ "s_select_argument list" 
+datatype s_query = SQ "s_select_argument list" s_from_argument s_where_argument s_group_by
 
 
-datatype s_table = ST "s_table_name * s_schema * ((s_rowname * s_value) list)"
+record s_table = 
+  table_name :: s_table_name
+  schema :: s_schema 
+  vals :: "(((s_rowname, s_value) fmap) list)"
 
-datatype s_insert_query = SIQ "(s_rowname * s_value) list"
+datatype s_insert_query = SIQ "(s_rowname, s_value) fmap"
 
-datatype s_database = SD "s_table list"
+datatype s_database = SD "(s_table_name, s_table) fmap"
 
 fun test_schema :: "unit \<Rightarrow> s_schema" where
-"test_schema _ = SS_Schema []"
+"test_schema _ = SS_Schema (
+  fmap_of_list 
+    [ (''id'', ST_Int)
+    , (''name'', ST_String)
+    ]
+)"
 
-value "test_schema ()"
+fun test_table :: "unit \<Rightarrow> s_table" where
+"test_table _ = 
+  \<lparr> table_name = STN_String ''test_table''
+  , schema = test_schema ()
+  , vals = []
+  \<rparr>
+" 
 
-inductive s_value_correct :: "s_value \<Rightarrow> s_type \<Rightarrow> bool" where
-svc_string : "s_value_correct (SV_String x) ST_String"
+fun test_db :: "unit \<Rightarrow> s_database" where 
+"test_db _ = SD (fmap_of_list [(STN_String ''test_table'', test_table ())])"
 
-inductive s_schema_correct :: "s_schema \<Rightarrow> s_insert_query \<Rightarrow> bool" where
-ssc_empty : "s_schema_correct (SS_Schema []) (SIQ [])" |
-ssc_cons : "s_schema_correct (SS_Schema x) (SIQ y) \<Longrightarrow> s_value_correct v t \<Longrightarrow> s_schema_correct (SS_Schema ((rn, t) # x)) (SIQ ((rn, v) # y))"
+value "SR_String ''a'' = SR_String ''b''"
+value "(case (test_schema ()) of 
+  SS_Schema x \<Rightarrow> fmdom x)"
 
-value "svc_string"
-(*inductive s_schema_correct :: *)
 
 fun is_value_correct :: "s_value \<Rightarrow> s_type \<Rightarrow> bool" where
 "is_value_correct (SV_String _) (ST_String) = True" |
+"is_value_correct (SV_Int _) (ST_Int) = True" |
+"is_value_correct (SV_Null) _ = True" |
 "is_value_correct _ _ = False"
 
-fun pop_from_map :: "s_rowname \<Rightarrow> (s_rowname * 'a) list \<Rightarrow> (( (s_rowname * 'a) list) * (s_rowname * 'a)) option" where
-"pop_from_map _ [] = None" |
-"pop_from_map (SRN_String s1) (((SRN_String s2), a) # xs) = (case s1 = s2 of
-  True \<Rightarrow> Some (xs, (SRN_String s1, a)) |
-  False \<Rightarrow> (case pop_from_map (SRN_String s1) xs of
-    Some (xs', v) \<Rightarrow> Some (((SRN_String s2), a) # xs', v) |
-    None \<Rightarrow> None))"
 
-(*lemma pop_smaller : "pop_from_map x y = Some (y', t) \<Longrightarrow> length y' < length y"
-  apply(induction y)
-  apply(auto)
-  done
-*)
+fun is_insert_query_correct_helper :: "s_schema \<Rightarrow> (s_rowname \<times> s_value) \<Rightarrow> bool" where
+"is_insert_query_correct_helper (SS_Schema sch) (rowname, value) = (
+  case fmlookup sch rowname of 
+    Some type_ \<Rightarrow> is_value_correct value type_ |
+    Empty \<Rightarrow> False
+)"
 
 fun is_insert_query_correct :: "s_schema \<Rightarrow> s_insert_query \<Rightarrow> bool" where
-"is_insert_query_correct (SS_Schema []) (SIQ []) = True" |
-"is_insert_query_correct (SS_Schema (x # xs)) (SIQ []) = False"|
-"is_insert_query_correct (SS_Schema y) (SIQ ((rn, v) # rest)) = (case pop_from_map rn y of
-  Some ((y', (rn', t))) \<Rightarrow> (is_value_correct v t \<and> is_insert_query_correct (SS_Schema y') (SIQ rest)) |
-  None \<Rightarrow> False)"
-by  auto
-termination by (relation "measures [\<lambda>(i, N). N, \<lambda>(i,N). N + 1 - i]") auto
+"is_insert_query_correct (SS_Schema sch) (SIQ iq) = (
+  let iq_set = fset_of_fmap iq; 
+      iq_dom = fmdom iq;
+      sch_dom = fmdom sch
+  in
+  fBall iq_set (is_insert_query_correct_helper (SS_Schema sch))
+  \<and> (HOL.equal iq_dom sch_dom)
+)"
 
-fun insert :: "s_insert_query \<Rightarrow> s_table \<Rightarrow> s_table option" where 
-"insert (SIQ "
+(*lemma is_insert_query_correct_same_no_of_args : "
+  is_insert_query_correct 
+    (SS_Schema (fmap_of_list [ (SR_String rn, t) ] )) 
+    (SIQ (fmap_of_list [ (SR_String rn, SV_Null) ])) 
+  = True" 
+  apply(induction t)
+  apply(auto)
+  done *)
+fun test_insert_query :: "unit \<Rightarrow> s_insert_query" where 
+"test_insert_query _ = SIQ (
+  fmap_of_list []
+)"
 
-fun test :: "unit \<Rightarrow> (string \<rightharpoonup>  int)" where
-"test _ = empty(''a'' \<mapsto>1)"
+value "is_insert_query_correct_helper (SS_Schema (fmap_of_list []))"
 
-value "test () ''a''"
+value "fBall (fset_of_list [True, False, True]) (\<lambda>x. x)"
+
+fun insert_to_table :: "s_insert_query \<Rightarrow> s_table \<Rightarrow> s_table option" where 
+"insert_to_table (SIQ iq) table = (
+  case is_insert_query_correct (schema table) (SIQ iq) of
+    False \<Rightarrow> None |
+    True \<Rightarrow> Some (table \<lparr> vals := (iq # (vals table)) \<rparr>)
+)"
+
+value "insert (test_insert_query ()) (test_table ())"
+
+fun select :: "s_query \<Rightarrow> s_database \<Rightarrow> s_query_result" where
+"select (SQ args from where groupby) (SD tables) = SQR_Error ''test'' "
+
 end 
